\begin{questions}

\question{Prove \textit{Lemma 7.23}. The product, maximum, and minimum of two simple functions are simple. The maximum of two functions f and g is defined by $(f \vee g)(x) = \max\{ f(x), g(x) \}$. The minimum of two functions f and g is defined by $(f \wedge g)(x) = \min\{ f(x), g(x) \}$}.

\begin{solution}
  \begin{proof}
Let $f, g : \Omega\rightarrow \R_+$ be simple (not necessarily in canonical representation),
\begin{align*}
f =\sum_{j=1}^m\alpha_j\chi_{A_j},~~g =\sum_{k=1}^n\beta_k\chi_{B_k}.
\end{align*}
We set
\begin{align*}
A=\bigcup_{j=1}^mA_j,~~B=\bigcup_{k=1}^nB_k,
\end{align*}
\begin{align*}
A_{m+1}=(A\cup B)\setminus A,~~B_{n+1}=(A\cup B)\setminus B,
\end{align*}
\begin{align*}
\alpha_{m+1} = 0 =\beta_{n+1}.
\end{align*}
Since $\mathcal{B}$ is a ring, $A$, $B$, $A\cup B$, and $A_{m+1}$ and $B_{n+1}$ are elements in $\mathcal{B}$.
Define
\begin{align*}
C_{jk}=A_j\cap B_k,~~j=1,...,m+1,~~k=1,...,n+1.
\end{align*}
Let $C_{jk}\neq\emptyset$ and note that for each $j,k$, $C_{jk}\in\mathcal{B}$. 
\begin{enumerate}[a)]
\item The product of two simple functions is a simple function.

The functions $f$ and $g$ can be expressed as
\begin{align*}
f=\sum_{j=1}^m\alpha_j\chi_{A_j}=\sum_{j=1}^{m+1}\alpha_j\sum_{k=1}^{n+1}\chi_{C_{jk}}=\sum_{j=1}^{m+1}\sum_{k=1}^{n+1}\alpha_j\chi_{C_{jk}},
\end{align*}
and
\begin{align*}
g=\sum_{k=1}^n\beta_k\chi_{B_k}=\sum_{k=1}^{n+1}\beta_k\sum_{j=1}^{m+1}\chi_{C_{jk}}=\sum_{j=1}^{m+1}\sum_{k=1}^{n+1}\beta_k\chi_{C_{jk}}.
\end{align*}
Therefore, the product $fg$ can be written as
\begin{align*}
fg=\sum_{j=1}^{m+1}\sum_{k=1}^{n+1}\alpha_j\beta_k\chi_{C_{jk}}.
\end{align*}
Thus, $fg$ can be written as a linear combination of indicator functions and therefore it is a simple function.
\item The maximum of two simple functions is a simple function.

The maximum of $f$ and $g$ can be expressed as follows:
\begin{align*}
(f \vee g)(x) &= \max\{ f(x), g(x) \}\\
&=\max\left\lbrace\sum_{j=1}^m\alpha_j\chi_{A_j}(x),\sum_{k=1}^n\beta_k\chi_{B_k}(x)\right\rbrace\\
&=\max\left\lbrace\sum_{j=1}^{m+1}\sum_{k=1}^{n+1}\alpha_j\chi_{C_{jk}}(x),\sum_{j=1}^{m+1}\sum_{k=1}^{n+1}\beta_k\chi_{C_{jk}}(x)\right\rbrace\\
&=\sum_{j=1}^{m+1}\sum_{k=1}^{n+1}\max\left\lbrace\alpha_j,\beta_k\right\rbrace\chi_{C_{jk}}(x)\\
&=\sum_{j=1}^{m+1}\sum_{k=1}^{n+1}\gamma_{jk}\chi_{C_{jk}}(x).
\end{align*}
Where we have made $\gamma_{jk}=\max\left\lbrace\alpha_j,\beta_k\right\rbrace$. Therefore,
\begin{align*}
(f \vee g)=\sum_{j=1}^{m+1}\sum_{k=1}^{n+1}\gamma_{jk}\chi_{C_{jk}},
\end{align*}
and as it happened before, $(f \vee g)$ can be written as a linear combination of indicator functions and therefore it is a simple function.

\item The minimum of two simple functions is a simple function.

The minimum of $f$ and $g$ can be expressed as follows:
\begin{align*}
(f \wedge g)(x) &= \min\{ f(x), g(x) \}\\
&=\min\left\lbrace\sum_{j=1}^m\alpha_j\chi_{A_j}(x),\sum_{k=1}^n\beta_k\chi_{B_k}(x)\right\rbrace\\
&=\min\left\lbrace\sum_{j=1}^{m+1}\sum_{k=1}^{n+1}\alpha_j\chi_{C_{jk}}(x),\sum_{j=1}^{m+1}\sum_{k=1}^{n+1}\beta_k\chi_{C_{jk}}(x)\right\rbrace\\
&=\sum_{j=1}^{m+1}\sum_{k=1}^{n+1}\min\left\lbrace\alpha_j,\beta_k\right\rbrace\chi_{C_{jk}}(x)\\
&=\sum_{j=1}^{m+1}\sum_{k=1}^{n+1}\delta_{jk}\chi_{C_{jk}}(x).
\end{align*}
Where we have made $\delta_{jk}=\min\left\lbrace\alpha_j,\beta_k\right\rbrace$. Therefore,
\begin{align*}
(f \wedge g)=\sum_{j=1}^{m+1}\sum_{k=1}^{n+1}\delta_{jk}\chi_{C_{jk}},
\end{align*}
and as it happened before, $(f \wedge g)$ can be written as a linear combination of indicator functions and therefore it is a simple function.
\end{enumerate}
\end{proof}
\end{solution}
\end{questions}