\begin{questions}

\question{Find the $L^2[-\pi,\pi]$ projection of the function
$f(x)=x^2$ onto the space $V_n\in L^2[-\pi,\pi]$ spanned by
\begin{align*}
\left\lbrace\frac{\sin(jx)}{\sqrt{2}\pi},\frac{\cos(jx)}{\sqrt{\pi}};j=1,2,...,n\right\rbrace
\end{align*}
for n=2. Plot these projections along with $f$ using a computer algebra
system. Repeat for $g(x)=x^3$.
}
\begin{solution}
Let $a_j=\frac{\sin(jx)}{\sqrt{2}\pi}$ and $b_j=\frac{\cos(jx)}{\sqrt{\pi}}$. Then, the projection, $f_0$, of $f$ onto the space $V_n$ is
\begin{align*}
f_0=\sum_{j=1}^n\left<f,a_j\right>a_j+\sum_{j=1}^n\left<f,b_j\right>b_j,
\end{align*}
where $n=2$. First, we calculate the inner products
\begin{align*}
\left<f,a_j\right>=\int_{-\pi}^{\pi}x^2\frac{\sin(jx)}{\sqrt{2}\pi}dx=\frac{1}{\sqrt{2}\pi}\int_{-\pi}^{\pi}x^2\sin(jx)dx=0,
\end{align*}
since $x^2\sin(jx)$ is odd. Thus,
\begin{align*}
\left<f,a_j\right>=0~~\forall j\in\Z.
\end{align*}
Now,
\begin{align*}
\left<f,b_j\right>=\int_{-\pi}^{\pi}x^2\frac{\cos(jx)}{\sqrt{\pi}}dx&=\frac{1}{\sqrt{\pi}}\int_{-\pi}^{\pi}x^2\cos(jx)dx\\
&=\frac{1}{\sqrt{\pi}}\cancelto{0}{\left.\frac{x^2\sin(jx)}{j}\right|_{-\pi}^{\pi}}-\frac{2}{\sqrt{\pi}}\int_{-\pi}^{\pi}\frac{1}{j} x\sin(jx)dx\\
&=-\frac{2}{j\sqrt{\pi}}\int_{-\pi}^{\pi}x\sin(jx)dx\\
&=+\frac{2}{j^2\sqrt{\pi}}\left.x\cos(jx)\right|_{-\pi}^{\pi}-\frac{2}{j^2\sqrt{\pi}}\int_{-\pi}^{\pi}\cos(jx)dx\\
&=+\frac{2}{j^2\sqrt{\pi}}\left.x\cos(jx)\right|_{-\pi}^{\pi}-\frac{2}{j^3\sqrt{\pi}}\cancelto{0}{\left.\sin(jx)\right|_{-\pi}^{\pi}}\\
&=+\frac{2}{j^2\sqrt{\pi}}\left(\pi\cos(j\pi)+\pi\cos(-j\pi)\right)\\
&=+\frac{4\sqrt{\pi}}{j^2}\cos(j\pi),
\end{align*}
where we have integrated by parts twice. Therefore,
\begin{align*}
f_0&=\cancelto{0}{\sum_{j=1}^n\left<f,a_j\right>a_j}+\sum_{j=1}^n\left<f,b_j\right>b_j\\
&=\left<f,b_1\right>b_1+\left<f,b_2\right>b_2\\
&=-4\sqrt{\pi}\frac{\cos(x)}{\sqrt{\pi}}+\sqrt{\pi}\frac{\cos(2x)}{\sqrt{\pi}}.
\end{align*}
Hence, the projection
\begin{align*}
f_0=\cos(2x)-4\cos(x).
\end{align*}
Further, we repeat the same process for the function $g(x)=x^3$. In this case, the parity of the function has changed from even to odd. Hence, in this case the inner products $\left<g,b_j\right>=0$ because $x^3\cos(jx)$ is an odd function.
We calculate then the inner products
\begin{align*}
\left<g,a_j\right>=\int_{-\pi}^{\pi}x^3\frac{\sin(jx)}{\sqrt{2}\pi}dx&=\frac{1}{\sqrt{2}\pi}\int_{-\pi}^{\pi}x^3\sin(jx)dx\\
&=-\frac{1}{\sqrt{2}\pi}\left.\frac{x^3\cos(jx)}{j}\right|_{-\pi}^{\pi}+\frac{1}{\sqrt{2}\pi}\frac{3}{j}\int_{-\pi}^{\pi}x^2\cos(jx)dx\\
&=-\frac{1}{j\sqrt{2}\pi}\left(\pi^3\cos(j\pi)+\pi^3\cos(-j\pi)\right)+\frac{3}{j\sqrt{2\pi}}\int_{-\pi}^{\pi}\frac{x^2\cos(jx)}{\sqrt{\pi}} dx\\
&=-\frac{2\pi^2}{j\sqrt{2}}\cos(j\pi)+\frac{3}{j\sqrt{2\pi}}\int_{-\pi}^{\pi}\frac{x^2\cos(jx)}{\sqrt{\pi}} dx\\
&=-\frac{\pi^2\sqrt{2}}{j}\cos(j\pi)+\frac{3}{j\sqrt{2\pi}}\frac{4\sqrt{\pi}}{j^2}\cos(j\pi)\\
&=\frac{6\sqrt{2}}{j^3}\cos(j\pi)-\frac{\pi^2\sqrt{2}}{j}\cos(j\pi).\\
\end{align*}
Similarly than with $f$, we have
\begin{align*}
g_0&=\sum_{j=1}^n\left<g,a_j\right>a_j+\cancelto{0}{\sum_{j=1}^n\left<g,b_j\right>b_j}\\
&=\left<g,a_1\right>a_1+\left<g,a_2\right>a_2\\
&=\sqrt{2}\left(\pi^2-6\right)\frac{\sin(x)}{\pi\sqrt{2}}+\frac{3-2\pi^2}{2\sqrt{2}}\frac{\sin(2x)}{\pi\sqrt{2}}\\
&=\frac{\left(\pi^2-6\right)}{\pi}\sin(x)+\frac{3-2\pi^2}{4\pi}\sin(2x)
\end{align*}
\end{solution}
\end{questions}
