\begin{questions}

\question{Show that the general solution to the heat equation 
\begin{displaymath}
	u(x, t) = \int_{-\infty}^\infty K(x -y, t) u_0(y) dy
\end{displaymath}
where the fundamental solution or kernel
\begin{displaymath}
	K(x, t) = \frac{1}{\sqrt{4 \pi \kappa t}} 
        \exp\left\{-\frac{x^2}{4 \kappa t}\right\}
\end{displaymath}
does in fact satisfy $u_t = \kappa \, u_{xx}$ with $u(x, t=0) =
u_0(x)$.  {\em Hint}: First show that $K$ satisfies the heat
equation. Then argue that $u$ satisfies the heat equation.  Finally show that $u$ satisfies the initial conditions $u(x, t=0) = u_0(x)$.
}
\begin{solution}
First we calculate the time derivative of $K$,
\begin{align*}
K_t(x,t)=\frac{x^2}{4\kappa\sqrt{4\kappa\pi}}\frac{e^{\frac{-x^2}{4\kappa t}}}{t^{5/2}}-\frac{1}{2\sqrt{4\kappa\pi}}\frac{e^{\frac{-x^2}{4\kappa t}}}{t^{3/2}}~.
\end{align*}
Further we calculate the spatial derivatives,
\begin{align*}
K_x(x,t)=-\frac{2x}{4\kappa t\sqrt{4\kappa\pi t}}e^{\frac{-x^2}{4\kappa t}},
\end{align*}
and
\begin{align*}
K_{xx}(x,t)=\frac{x^2}{4\kappa^2\sqrt{4\kappa\pi}}\frac{e^{\frac{-x^2}{4\kappa t}}}{t^{5/2}}-\frac{1}{2\kappa\sqrt{4\kappa\pi}}\frac{e^{\frac{-x^2}{4\kappa t}}}{t^{3/2}}~.
\end{align*}
Finally, it is easy to check that
\begin{align*}
\kappa K_{xx}=\frac{x^2}{4\kappa\sqrt{4\kappa\pi}}\frac{e^{\frac{-x^2}{4\kappa t}}}{t^{5/2}}-\frac{1}{2\sqrt{4\kappa\pi}}\frac{e^{\frac{-x^2}{4\kappa t}}}{t^{3/2}}=K_t(x,t),
\end{align*}
and that $K$ satisfies the heat equation.
Now it is easier to check that $u$ satisfies it as well,
\begin{align*}
\kappa u_{xx}&=\kappa\frac{\partial^2}{\partial x^2}\int_\infty^{\infty}K(x -y, t) u_0(y) dy\\
&=\int_\infty^{\infty}\kappa K_{xx}(x -y, t) u_0(y) dy\\
&=\int_\infty^{\infty} K_{t}(x -y, t) u_0(y) dy\\
&=\frac{\partial}{\partial t}\int_\infty^{\infty}K(x -y, t) u_0(y) dy\\
&=\frac{\partial}{\partial t}u(x,t)\\
&=u_t.
\end{align*}
To check that the initial condition is satisfied by this solution we take the limit,
\begin{align*}
\lim_{t\to 0}u(x,t)&=\lim_{t\to 0}\int_{-\infty}^\infty K(x -y, t) u_0(y) dy\\
&=\int_{-\infty}^\infty \lim_{t\to 0}K(x -y, t) u_0(y) dy\\
&=\int_{-\infty}^\infty \delta(x-y) u_0(y) dy\\
&=u_0(x),
\end{align*}
where we have used the fact that the limit at time zero of the heat kernel is the Dirac delta and its properties.
\end{solution}
\end{questions}
