{\bf E 5.3.2}. Let $G$ be the GF. Show: $G(x,y,t+r)=\int_0^L G(x,z,t)G(z,y,r) dz, 0 \leq x,y\leq L, t,r \geq 0$. There are several ways to prove this.  One way is to use the Fourier sine representation formula and orthonormality.  Another is to fix $r$ and, for fixed by arbitrary cont $f: [0,L] \ra \R$ with $f(0)=0=f(L)$ consider $u(x,t)=\int_0^L G(x,y,t+r)f(y)dy$ and $v(x,t)=\int_0^L G(x,z,t)g(z)dz$ with $g(x)=\int_0^LG(x,y,r)f(y)dy$. {\it Proof}. Recall that $G(x,y,t) = \sum_{m=1}^{\infty} (2/L) \sin(\lambda_mx) \sin(\lambda_m y) e^{-a\lambda_m^2 t}$. Then $\int_0^L G(x,z,t) G(z,y,r) dz = (2/L) \sum_{m=1}^{\infty}\sin(\lambda_mx)  e^{-a \lambda_m^2 t}\sum_{m=1}^{\infty} [(2/L) \int_0^L \sin(\lambda_mz) \sin(\lambda_k z) dz] \sin(\lambda_ky)  e^{-a\lambda_k^2 r})$. Because of orthonormality, the integrals in the brackets are 0 if $k \neq m$ and 1 if $k=m$. Then $\int_0^L G(x,z,t)G(z,y,r) dz$ = $(2/L) \sum_{m=1}^{\infty} \sin(\lambda_mx)  e^{-a\lambda_m^2 t} \sin(\lambda_my)  e^{-a\lambda_m^2 r}= (2/L) \sum_{m=1}^{\infty} \sin(\lambda_m x) \sin(\lambda_m y)  e^{-a\lambda_m^2 (t+r)}=G(x,y,t+r) \qed$