{\bf E9.1.5} Let $\Gamma$ be the fund soln of the HE in 1 space dim defined by (9.2). Let $b: \R_+ \ra \R$ and $a: \R_+ \ra \R$ be cont. Let $B(t) = \int_0^t b(s) ds$ and $A(t) = \int_0^t a(s) ds$. Assume $A(t) > 0\; \forall \; t>0$. Define $\tilde{\Gamma} (t,x) = \Gamma(x+B(t), A(t)), x \in \R, t>0$. (a) Show that $\partial_t \tilde{\Gamma}(t,x) = b(t)\partial_x\tilde{\Gamma}(t,x) + a(t) \partial_x^2 \tilde{\Gamma}(t,x)$. (b) Show that $\int_{\R}\tilde{\Gamma}(t,x)dx=1, \int_{\R}x \tilde{\Gamma}(t,x)dx=-B(t)$ and $\int_{\R} (x+ B(t))^2\tilde{\Gamma}(t,x)dx=2 A(t)$. 
%(This means that, for any $t>0, \tilde{\Gamma}(t, \cdot)$ is the probability density of a normal distribution with mean $-B(t)$ and variance $2A(t)$.) Remark:  As you notice, notation for the fundamental solution is not consistent as to whether the space variable come first or the time variable. 
{\it Prf}. (a) By the chain rule and the fund thm of calc, $\partial_t \tilde{\Gamma}(t,x) = \partial_1 \Gamma(x + B(t), A(t))b(t) + \partial_2 \Gamma(x + B(t), A(t))a(t)$. Again, by the chain rule, and by the PDE for $\Gamma, \partial_t \tilde{\Gamma}(t,x) = b(t) \partial_x \Gamma(x+B(t), A(t)) + a(t) \partial_1^2 \Gamma(x+B(t), A(t))$. Use chain rule, $\partial_t \tilde{\Gamma}(t,x) = b(t)\partial_x \tilde{\Gamma}(t,x) + a(t) \partial_x^2 \Gamma(x+B(t), A(t)) = b(t)\partial_x \tilde{\Gamma}(t,x) + a(t) \partial_x^2 \tilde{\Gamma}(t, x)$. (b) Subst $x = y - B(t), \int_{\R} \tilde{\Gamma}(t,x) dx$ = $\int_{\R} \Gamma (x + B(t), A(t)) dx$ = $\int_{\R}\Gamma(y, A(t))dy = 1, \int_{\R} x \tilde{\Gamma}(t,x) dx$ = $ \int_{\R} x \Gamma (x + B(t), A(t)) dx$ = $\int_{\R}(y-B(t))\Gamma(y, A(t))dy$ = $\int_0^{\infty} y \Gamma (y, A(t))dy - \int_0^{\infty} y \Gamma (-y, A(t))dy - B(t) \int_{\R} \Gamma(y, A(t))dy$. Since $\Gamma( -y, A(t)) = \Gamma (y, A(t))$ and $\int_{\R} \Gamma(y, A(t))dy = 1$, the assertion follows.  Finally, $V(t) := \int_{\R} (x + B(t))^2 \tilde{\Gamma} (t,x) dx$ = $\int_{\R} (x + B(t))^2 \Gamma (x + B(t), A(t)) dx$ = $\int_{\R} y^2 \Gamma (y, A(t)) dy = \int_{\R} y^2 (4 \pi A(t))^{-1/2} e^{-y^2(4A(t))^{-1}} dy$.  We substitute $y = (4 A(t))^{1/2} z$ and IBP, $V(t) = (\pi)^{-1/2} 4 A(t) \int_{\R} z^2 e^{-z^2}dz = - (\pi)^{-1/2} 2 A(t) \int_{\R} z (d/dz) e^{-z^2}dz$ = $- (\pi)^{-1/2} 2 A(t) \int_{\R} z  e^{-z^2}dz]_{z = - \infty}^{z = \infty} +  (\pi)^{-1/2} 2 A(t) \int_{\R} z  e^{-z^2}dz = 2 A(t) \qed$