{\bf P9.6}. Define $G(x,t) = \Pi_{i=1}^n \Gamma(x_i, t), t >0, x = (x_1, \dots, x_n) \in \R^n$. Then: (a) $\partial_t G(x,t) = \Delta_x G(x,t), t > 0, x \in \R^n$.  (b) $\int_{\R^n} G(x,t) dx = 1\; \forall \; t > 0$. (c) $G(x,t) = (4 \pi t)^{-n/2} e^{-||x||^2(4t)^{-1}}$, where $|| \cdot ||$ is the Euclidean norm on $\R^n$. (d) For every $\epsilon > 0, \int_{||x|| \geq \epsilon} G(x,t) dx \ra 0$ as $t \ra 0$. (e) (Chapman-Kolmogorov eq) $\forall \; t,r \in [0, \infty), x \in \R^n, G(x,t+r) = \int_{\R^n} G(x-y, t) G(y,r)dy$. {\it Prf}. (a) By the product rule, $\partial_t G(x,t) = \sum_{j=1}^n ( \Pi_{i \neq j} \Gamma (x_i, t))\partial_t \Gamma(x_j,t)$ = $\sum_{j=1}^n ( \Pi_{i \neq j} \Gamma (x_i, t))\partial_{x_j}^2 \Gamma(x_j,t)$ = $ \sum_{j=1}^n \partial_{x_j}^2 ( \Pi_{i \neq j} \Gamma (x_i, t))\Gamma(x_j,t)$  = $\Delta_x G(x,t)$. (b) We use induction over $n$. Write $G_n$ for $G$. We know the statement to be true for $n =1$. Let $n \in \N$ be arbitrary and assume that the statement is true for $n$. Notice that, for $y \in \R^n$ and $z \in \R, G_{n+1}((y,z),t) = G_n(y,t)\Gamma(z,t)$. Now, by the thms of Fubini or Tonelli, $\int_{\R^{n+1}} G_{n+1}(x, t) dx$ = $ \int_{\R^n} \int_{\R} G_n (y, t) \Gamma (z, t) dy dz$ = $( \int_{\R} G_n (y, t) dy)(\int_{\R} \Gamma (z, t) dz) = 1 \cdot 1 = 1$. (c) $G(x, t) = \Pi_{i=1}^n ((4 \pi t)^{-1/2} e^{-x_i^2(4t)^{-1}})$ = $(4 \pi t)^{-n/2} \Pi_{i=1}^n e^{-x_i^2(4t)^{-1}}$ = $(4 \pi t)^{-n/2} \exp ( - \sum_{i=1}^n x_i^2 (4t)^{-1})$ = $(4 \pi t)^{-n/2} e^{-||x||^2(4t)^{-1}}$. (d) Let $\epsilon > 0$. We substitute $x = t^{1/2}y, \int_{||x||\geq \epsilon} G(x,t)dx$ = $(4 \pi )^{-n/2} \int_{||y||\geq \epsilon t^{-1/2}} e^{-||y||^2 /4}$ = $\int_{||y||\geq \epsilon t^{-1/2}} G(y,1) dy \ra 0$, as $t \ra 0$. (e) Let $t, r \in [0, \infty), x \in \R^n. \int_{\R^n} G(x-y, t) G(y,r) dy$ = $ \int_{\R^n} \Pi_{j=1}^n \Gamma(x_j - y_j, t) \Pi_{j=1}^n \Gamma(y_j, r) dy$ = $\int_{\R^n} \Pi_{j=1}^n [\Gamma(x_j - y_j, t)  \Gamma(y_j, r) ]dy$ = $  \Pi_{j=1}^n \int_{\R} [\Gamma(x_j - y_j, t)  \Gamma(y_j, r) ]dy_j$ = $ \Pi_{j=1}^n \Gamma(x_j. t+r) = G(x,t+r) \qed$