{\bf T5.21}. If $u$ is a soln of (5.35) and $u$ and $F$ are cont and bdd on $[0,L] \times (0, T)$, then $u(x, t) = \int_0^L G(x,y,t)f(y)dy+\int_0^t \int_0^L G(x,y,s)F(y,t-s)dsdy, 0<t<T, 0\leq x \leq L$. Under which assumptions for $F$ is this a soln? Since we already studied the homog IVP in detail, we can set $f=0$ and, after a subst, set $\tilde{u}(x,t)=\int_0^t \int_0^L G(x,y,t-s)F(y,s)dsdy$ (5.36). Interchanging int and the series rep of $G$, (5.27), we obtain the Fourier sin rep, $\tilde{u}(x,t)=\sum_{m=1}^{\infty} \tilde{u}_m(x,t), \tilde{u}_m(x,t)$ = $\sin(\lambda_m x)(2/L)\int_0^t \int_0^L \sin(\lambda_m y)e^{-a \lambda_m^2(t-s)} F(y,s)dsdy$ = $\sin(\lambda_m x) e^{-a \lambda_m^2 t} (2/L)\int_0^t e^{a \lambda_m^2 s}(\int_0^L \sin(\lambda_m y) F(y,s)dy)ds$ (5.37).  
%We could have also obtained this expression directly from expanding $\tilde{u}$ and $F$ into Fourier sine series and deriving ODEs for the Fourier coeffs of $\tilde{u}$ involving the Fourier coeffs of $F$ (E 5.4.1).
We have the est $|\tilde{u}_m(x,t)|\leq 2 \sup |F| \int_0^t e^{-a \lambda_m^2(t-s)}ds$
$\leq (2\sup|F|)/(a \lambda_m^2)$. Since the series over the rhs converges (recall that $\lambda_m$ is proportional to $m$), the series for $\tilde{u}$ converges unif on $[0,L] \times [0,T]$ and $\tilde{u}$ is cont on $[0,L] \times [0,T], \tilde{u}(x,0) = 0\; \forall \; x \in [0,L]$. By the product rule and the fund thm of calc, $\partial_t \tilde{u}_m(x,t)$ = $-a \lambda_m^2 \tilde{u}_m(x,t) + \sin(\lambda_m x) (2/L) \int_0^L \sin (\lambda_m y) F(y, t) dy$ (5.38)  $=a \partial_x^2 \tilde{u}_m(x,t) + \sin ( \lambda_m x) (2/L) \int_0^L \sin(\lambda_m y) F(y, t) dy$ (5.39). We make a change of variables in the int for $\tilde{u}_m$ in (5.37),  $\partial_t \tilde{u}_m(x,t) = -a \lambda_m^2  \sin(\lambda_m x) (2/L) \int_0^t \int_0^L \sin(\lambda_m y) e^{-a \lambda_m^2 s} F(y,t-s)dy ds +\sin(\lambda_m x) (2/L) \int_0^L \sin(\lambda_m y) F(y,t)dy$ (5.40). We change the order of int and combine the spatial ints, $\partial_t \tilde{u}_m(x,t)$ = $\sin(\lambda_m x) (2/L) \int_0^L \sin(\lambda_m y) H(y,t)dy, H(y,t) = -a \lambda_m^2  \int_0^t  e^{-a \lambda_m^2 s}$
$F(y,t-s)ds + F(y,t)$. Since $a \lambda_m^2  \int_0^t  e^{-a \lambda_m^2 s} ds = 1 - e^{-a \lambda_m^2 t}, H(y,t)=a \lambda_m^2  \int_0^t  e^{-a \lambda_m^2 s} [F(y,t) - F(y,t-s)]ds -a \lambda_m^2  \int_0^t  e^{-a \lambda_m^2 s} ds F(y,t)+ F(y,t) =a \lambda_m^2  \int_0^t  e^{-a \lambda_m^2 s} [F(y,t) - F(y,t-s)]ds + e^{-a \lambda_m^2 t} F(y,t)$.  Assume $F$ is Lip cont in the time var:  $\exists \; \Lambda >0$ s.t. $|F(y,t)- F(y,s)| \leq \Lambda|t-s|, 0 \leq y \leq L, 0\leq s,t \leq T$. Then $|H(y,t)| \leq a \lambda_m^2  \int_0^t  e^{-a \lambda_m^2 s} \Lambda s ds + e^{-a \lambda_m^2 t} |F(y,t)|$. Subst $r=a \lambda_m^2 s, |H(y,t)| \leq (L/(a \lambda_m^2) \int_0^{ta\lambda_m^2}e^{-r} r dr + e^{-a\lambda_m^2t} |F(y,t)| \leq  (L/(a \lambda_m^2) + e^{-a\lambda_m^2t} |F(y,t)|$. Now $|\partial_t \tilde{u}_m(x,t)| \leq | \sin(\lambda_m x)| (2/L) \int_0^L $
$| \sin(\lambda_my)| |H(y,t)| dy \leq (2/L) \int_0^L  |H(y,t)| dy $. Sub est $|H(y,t)|, |\partial_t\tilde{u}_m(x,t)|\leq (2 \Lambda)/(a \lambda_m^2) + e^{-a\lambda_m^2t} (2/L) \int_0^L  |F(y,t)| dy$ (5.41). By T5.3, $u$ is PD wrt $t$ on $[0,L] \times (0, T]$ and $\partial_t u = \sum_{m=1}^{\infty}\partial_t \tilde{u}_m$ with the series converging unif on $[0,L] \times [\epsilon, T]$ for every $\epsilon \in (0,T)$. Similarly one shows that $u$ is twice PD wrt $x$ and $\partial_x^2 u = \sum_{m=1}^{\infty}\partial_x^2 \tilde{u}_m$ with the series converging unif on $[0,L] \times [\epsilon, T]$ for every $\epsilon \in (0,T)$.By (5.39), $\partial_t \tilde{u} - a \partial_x^2\tilde{u} = \sum_{m=1}^{\infty}\sin(\lambda_mx) (2/L) \int_0^L \sin(\lambda_my) F(y,t) dy$. where the convergence on the rhs is unif on $[0,L] \times [\epsilon, T]$ for every $\epsilon \in (0,T)$. Since the sines form an orthonormal basis, the rhs equals the Fourier sine series of $F(\cdot, t)$ and so equals $F(x,t)$ for a.a. $x$. Further, for fixed $t$, the convergence holds in $L^2[0,L]$ wrt the space var.  Since both $\partial_t \tilde{u} - a \partial_x^2\tilde{u} $ and $F$ are cont, $\partial_t \tilde{u} - a \partial_x^2\tilde{u} = F$. Further $\tilde{u}(x,0) = 0$ and $\tilde{u}(0,t) = 0 = \tilde{u}(L,t)$. 