\begin{questions}

\question{ Let $X$ be a metric space with metric $d$ and $S$ and $T$ be subsets of $X$. 

Show: $int(S \cap T) = \breve{S} \cup \breve{T}$}

\begin{solution}
  \begin{proof}
 Observe that,
\begin{align*}
X \setminus  (\breve{S} \cap \breve{T}) = X \setminus \breve{S} ~\cup ~X \setminus \breve{T}
\end{align*} 
 By DeMorgan's law. 
 
 Then, by proposition 4.17,
 \begin{align*}
X \setminus \breve{S} ~\cup ~X \setminus \breve{T} = \overline{X \setminus S}~\cup~\overline{X \setminus T}~ = \overline{X \setminus S~\cup~X \setminus T }~.
 \end{align*}
 Then, by DeMorgan's Law and proposition 4.17,
 \begin{align*}
 \overline{X \setminus S~\cup~X \setminus T } = \overline{X \setminus S \cap T} = X \setminus Int(S \cap T)~.
 \end{align*}
 Thus,
 \begin{align*}
 &X \setminus  (\breve{S} \cap \breve{T}) = X \setminus Int(S \cap T)
 \\
 & \Rightarrow \breve{S} \cap \breve{T} = Int(S \cap T)~.
 \end{align*}
  \end{proof} 
\end{solution}

\question{$\breve{S} \cup \breve{T} \subseteq Int(S \cup T)$ but equality fails in general. } 

\begin{solution}
  \begin{proof}
  
Let $x \in  \breve{S} \cap \breve{T}$. Then,

Case 1: Let $x \in \breve{S}$, $\exists~ \varepsilon_1>0$ such that,
\begin{align*}
U_{\varepsilon_1}(x) \subseteq S \subseteq S \cup T~.
\end{align*}
Thus $x \in Int(S \cup T)$.
\vspace{5mm}

Case 2: Let $x \in \breve{T}$, $\exists~ \varepsilon_2>0$ such that,
\begin{align*}
U_{\varepsilon_2}(x) \subseteq T \subseteq S \cup T~.
\end{align*}
Thus, $x \in Int(S \cup T)$.
\vspace{5mm}

Case 3: Let $x \in \breve{S} \cup \breve{T}$, $\exists \varepsilon_3>0$ such that,
\begin{align*}
U_{\varepsilon_3}(x) \subseteq S \cap T \subseteq S \cup T~.
\end{align*}
Thus, $x \in Int(S \cup T)$.
\vspace{5mm}

Then $x \in \breve{S}\cap \breve{T} \Rightarrow x \in Int(S \cup T)$. Thus,
\begin{align*}
\breve{S} \cup \breve{T} \subseteq Int(S \cup T)
\end{align*}
\vspace{7mm}

Now, lets show that equality fails in general. Let $(\R, d)$ be the real number line under Euclidean topology.   Let $S = [a, \cdots, b]$ and $T = [b, \cdots, c] ~\forall~~a,b,c \in \R$. Then,
\begin{align*}
Int(S \cup T) &= Int([a, \cdots, b] \cup [b, \cdots, c])\\
& = Int([a, \cdots, c]) \\
& = (a, \cdots, c)~,
\end{align*}
and
\begin{align*}
\breve{S} \cup \breve{T} &= Int([a, \cdots, b]) \cup Int([b, \cdots, c]) \\
& = (a, \cdots, b) \cup (b, \cdots, c) \\
& \neq (a, \cdots, c)~.
\end{align*}
Thus, the equality fails.

  \end{proof} 
\end{solution}

\end{questions}