{\bf Exercise 5.2.6}. (a) Find the sol $w$ of $-\partial_x^2 w(x)=2, \quad 0<x<1, w(0) = 0 = w(1).$ (b) Suppose that $u$ is the sol to $(\partial_t - \partial_x^2)u=2 \quad \text{ on } (0,1) \times (0, \infty), u(0,t)=0=u(1,t), \quad t \geq 0, u(x,0)=0, \quad 0 \leq x \leq 1.$ Show that 
$x(1-x)(1-e^{-8t})\leq u(x,t) \leq x(1-x), \quad 0 \leq x \leq 1.$ Remark:  $w$ in part (a) is the steady state for the equation in part (b). {\it Proof}. (a) We integrate twice to get
$\partial_x w(x)=-2x+c_1 \implies w(x)=-x^2+c_1+c_2$. Now we check boundary conditions. $w(0)=0=c_2$ and $w(1)=0=-1+c_1$ and so we have that $c_1 = 1$ and so $w(x)=-x^2+x=x(1-x)$. (b) We let $v(x,t)=x(1-x)(1-e^{-8t})$.  Then $\partial_t v(x,t)=x(1-x)8e^{-8t}$ and $\partial_x v(x,t)=-2x(1-e^{-8t})$ and $\partial_x^2=-2(1-e^{-8t})$.  We put this together to get $(\partial_t - \partial_x^2)v=x(1-x)8e^{-8t}+2(1-e^{-8t})=2[4x(1-x)e^{-8t}+(1-e^{-8t})]=2[e^{-8t}(4x(1-x)-1)+1]$.  Given that $f(x)=x(1-x), f'(x)=1-2x=0$ at $x=1/2$ and so $f(x)$ has a max at $1/4$.  So  $2[e^{-8t}(4x(1-x)-1)+1] \leq 2[e^{-8t}(4(1/4)-1)+1]=2$
Therefore $(\partial_t-\partial_x^2)v \leq 2$.  Now we set $\tilde{v}=v-u$. Then $(\partial_t - \partial_x^2) \tilde{v}=(\partial_t-\partial_x^2)v-(\partial_t-\partial_x^2)u \leq 2-2=0$.  Further, for $\partial \Omega = \{0,1\}, \tilde{v}(0,t)=(v-u)(0,t)=v(0,t)-u(0,t)=0(1-0)(1-e^{-8t})-0=0, t \geq 0$ and $\tilde{v}(1,t)=(v-u)(1,t)=v(1,t)-u(1,t)=1(1-1)(1-e^{-8t})-0=0, t \geq 0$ and $\tilde{v} (x,0) = (v-u)(x,0) = v(x,0)-u(x,0)=x(1-x)(1-1)-0=0, \; 0 \leq x \leq 1.$ So we have $(\partial_t -\partial_x^2)\tilde{v} \leq 0, \text{ on } (0,1)\times (0,\infty), \tilde{v}(0,t) = 0 = \tilde{v} (1,t) \quad t \geq 0, \tilde{v}(x,0)=0 \quad 0 \leq x \leq 1.$ By T 5.11, $\tilde{v} \leq 0$ and therefore $v \leq u$.  Now, recall $w$ from part (a).  Set $\tilde{w}=u-w$. Then 
$(\partial_t-\partial_x^2)\tilde{w}=(\partial_t-\partial_x^2)u-(\partial_t-\partial_x^2)w = 2-2=0$.  Further, for $\partial \Omega = \{0,1\}, \tilde{w}(0,t)=u(0,t)-w(0,t)=0-0=0, t \geq 0$ and $\tilde{w} (1,t) =u(1,t)-w(1,t)=0-0=0, t \geq 0$ and $\tilde{w}(x,0)=u(x,0)-w(x,0)=0-x(1-x) \leq 0, \; 0 \leq x \leq 1.$ And so we have $(\partial_t - \partial_x^2)\tilde{w}=0$ on $(0,1)\times (0,\infty), \tilde{w}(0,t)=0=\tilde{w}(1,t), t \geq 0, \tilde{w}(x,0) \leq 0, 0 \leq x \leq 1$. So by T 5.11, we have that $\tilde{w} \leq 0$ and so $u \leq w$ and so $v \leq u \leq w, 0 \leq x \leq 1\qed$.