\begin{questions}

\question{In the modified PDE for the Lax-Wendroff method for $u_t + c u_x =
0$, derive the coefficient $\beta = \frac{c h^2}{6} (r^2 - 1)$ of
numerical dispersion in $u_t + c u_x = \beta u_{xxx}$.
}
\begin{solution}
We start by Taylor expanding 
\begin{align*}
u^{n+1}_j&=u_j^n+\Delta t u_t+\frac{\Delta t^2}{2} u_{tt}+\frac{\Delta t^3}{6} u_{ttt}+\mathcal{O}(\Delta t^4),\\
u^{n}_{j\pm 1}&=u_j^n\pm\Delta x u_x+\frac{\Delta x^2}{2} u_{xx}\pm\frac{\Delta x^3}{6} u_{xxx}+\mathcal{O}(\Delta x^4),
\end{align*}
and substituting them (neglecting the higher order terms) into the Lax-Wendroff scheme,
\begin{align*}
u_j^{n+1}&=u_j^n-\frac{c\Delta t}{2\Delta x}\left(u^n_{j+1}-u^n_{j-1}\right)+\frac{c^2\Delta t^2}{2\Delta x^2}\left(u^n_{j+1}-2u^n_{j}+u^n_{j-1}\right),\\
u_j^n+\Delta t u_t+\frac{\Delta t^2}{2} u_{tt}+\frac{\Delta t^3}{6} u_{ttt}&=u_j^n-\frac{c\Delta t}{2\Delta x}\left(2\Delta x u_x+\frac{\Delta x^3}{3} u_{xxx}\right)+\frac{c^2\Delta t^2}{2\Delta x^2}\Delta x^2 u_{xx}.
\end{align*}
Doing some algebraic manipulations we reach,
\begin{align*}
u_t+cu_x=-\frac{\Delta t}{2} u_{tt}-c\frac{\Delta x^2}{6}u_{xxx}+\half c^2\Delta t u_{xx}-\frac{\Delta t^2}{6}u_{ttt}.
\end{align*}
Using the original PDE we obtain that
\begin{align*}
u_t=-cu_x&\Rightarrow u_{tt}=c^2u_{xx},\\
&\Rightarrow u_{ttt}=-c^3u_{xxx}.
\end{align*}
Hence,
\begin{align*}
u_t+cu_x&=-\frac{\Delta t}{2} c^2u_{xx}-c\frac{\Delta x^2}{6}u_{xxx}+\half c^2\Delta t u_{xx}+\frac{\Delta t^2}{6}c^3u_{xxx},\\
&=-c\frac{\Delta x^2}{6}u_{xxx}+\frac{\Delta t^2}{6}c^3u_{xxx},\\
&=c\frac{\Delta x^2}{6}\left(\frac{c^2\Delta t^2}{\Delta x^2} -1\right)u_{xxx},\\
&=c\frac{\Delta x^2}{6}\left(r^2 -1\right)u_{xxx},\\
&=\beta u_{xxx}.
\end{align*}
\end{solution}
\end{questions}
