{\bf Properties:} 
\begin{itemize}
\item $\mathcal{F}[\alpha f+\beta g]=\alpha \mathcal{F}[f]+\beta \mathcal{F}[g]$ // $\mathcal{F}^{-1}[\alpha f+\beta g]=\alpha \mathcal{F}^{-1}[f]+\beta \mathcal{F}^{-1}[g]$
\item $\mathcal{F}[t^nf(t)](\lambda)=i^n\frac{d^n}{d\lambda^n}\{\mathcal{F}[f](\lambda)\}$
\item $\mathcal{F}^{-1}[\lambda^nf(\lambda)]........(t)=(-i)^n\frac{d^n}{dt^n}\{\mathcal{F}^{-1}[f](t)\}$
\item $\mathcal{F}[f^{(n)}(t)](\lambda)=(i\lambda)^n\mathcal{F}[f](\lambda)$
\item $\mathcal{F}^{-1}[f^{(n)}(\lambda)](t)=(-it)^n\mathcal{F}^{-1}[f](t)$
\item $\mathcal{F}[f(t-a)](\lambda)=e^{-i\lambda a}\mathcal{F}[f](\lambda)$
\item $\mathcal{F}[f(bt)](\lambda)=\frac{1}{b}\mathcal{F}[f](\frac{\lambda}{b})$
\item If $f(t<0)=0$, then $\mathcal{F}[f](\lambda)=\frac{1}{\sqrt{2\pi}}\mathcal{L}[f](i\lambda)$, where \newline $\mathcal{L}[f](s)=\int_0^{\infty}f(t)e^{-ts}dt$.
\end{itemize}