In this section we will show the finite difference equations needed to solve
\begin{align*}
\frac{\partial u}{\partial t}=\frac{1}{Re}\left(\frac{\partial^2 u}{\partial x^2}+\frac{\partial^2 u}{\partial y^2}\right),
\end{align*}
using ADI. Let $d_1=\frac{\Delta t}{2Re\Delta x^2}$ and $d_2=\frac{\Delta t}{2Re\Delta y^2}$.
\subsection{Step 1. Implicit in x-direction}
The differential equation discretized implicitly in the x-direction yields
\begin{align*}
\frac{u_{i+1/2,j}^{n+1/2}-u_{i+1/2,j}^n}{\Delta t/2}=\frac{1}{Re\Delta x^2}\left(u_{i+3/2,j}^{n+1/2}-2u_{i+1/2,j}^{n+1/2}+u_{i-1/2,j}^{n+1/2}\right)+\frac{1}{Re\Delta y^2}\left(u_{i+1/2,j+1}^{n}-2u_{i+1/2,j}^{n}+u_{i+1/2,j-1}^{n}\right).
\end{align*}
Using the definitions of $d_1$, $d_2$ and reorganizing the terms we obtain
\begin{align*}
-d_1u_{i-1/2,j}^{n+1/2}-(1+2d_1)u_{i+1/2,j}^{n+1/2}-d_1u_{i+3/2,j}^{n+1/2}=d_2u_{i+1/2,j-1}^n+(1-2d_2)u_{i+1/2,j}^n+d_2u_{i+1/2,j+1}^n,
\end{align*}
which gives us
\begin{align*}
a_{i+1/2,j}=-d_1,~~~~~~b_{i+1/2,j}=1+2d_1,~~~~~~c_{i+1/2,j}=-d_1,
\end{align*}
and
\begin{align*}
d_{i+1/2,j}=d_2u_{i+1/2,j-1}^n+(1-2d_2)u_{i+1/2,j}^n+d_2u_{i+1/2,j+1}^n.
\end{align*}
\subsubsection{Boundary Conditions}
To account for the left boundary we have imposed $a_{3/2,j}=0$ and 
\begin{align*}
d_{3/2,j}=d_2u_{3/2,j-1}^n+(1-2d_2)u_{3/2,j}^n+d_2u_{3/2,j+1}^n+d_1u_{3/2,j},
\end{align*}
where $u_{3/2,j}$ is given by the boundary conditions

\[ u_{3/2,j}=\begin{cases} 
      U_{in1}(y_j) & x\leq 0 \\
      0 & 100\leq x 
   \end{cases}
\]

\subsection{Step 2. Implicit in y-direction}
