{\bf Identities:} $\sin^2x = (1-\cos 2x)/2, \cos^2x = (1+\cos 2x)/2$, $e^{ix}=\cos x + i \sin x, e^{-ix}=\cos x - i \sin x$,  \newline$e^{ix}+e^{-ix}=2\cos x$,\newline $e^{ix}-e^{-ix}=2i\sin x$. \newline%$2 \cosh x=(e^x+e^{-x}), 2\sinh x=(e^x-e^{-x}). \cosh^2 x-\sinh^2x=1$. \newline
{\bf Sum and Difference Formula:} $\sin(A\pm B)=\sin A \cos B\pm \cos A \sin B$. $\cos(A\mp B)=\cos A \cos B\pm \sin A \sin B$. $\tan(A \pm B)=(\tan A\pm \tan B)/(1\mp \tan A \tan B)$. \newline
{\bf Double Angle Formula:}  $\sin(2A)=2 \sin A \cos A$. $\cos(2A)=\cos^2 A-\sin^2 A=2 \cos^2 A-1=1-2\sin^2 A$. $\tan(2A)=(2\tan A)/(1-\tan^2 A)$.  \newline
%{\bf Half Angle Formula:} $\sin(A/2)=\pm \sqrt{(1-\cos A)/2}$. $\cos(A/2)=\pm \sqrt{(1+\cos A)/2}$. \newline
%{\bf Product to Sum:} $\cos A \cos B=(1/2)(\cos(A+B)+\cos(A-B))$. $\sin A \sin B=(1/2)(\cos(A-B)-\cos(A+B)$. $\sin A \cos B=(1/2)(\sin(A+B)+\sin(A-B)$.  \newline
{\bf Sum to Product:} $\sin A\pm \sin B=2\sin((A\pm B)/2)\cos((A\mp B)/2)$. $\cos A - \cos B=-2\sin((A+B)/2)\sin((A-B)/2)$. $\cos A + \cos B=2\cos((A+B)/2)\cos((A-B)/2)$. \newline
{\bf Geometric Sum:} $\sum_{k=0}^N z^k=\frac{1-z^{N+1}}{1-z}$. $\sum_{k=0}^{\infty}z^k=\frac{1}{1-z}$.  \newline
%{\bf General ODE Solutions:}  $y''=y(t)\implies y=c_1e^{-t}+c_2e^t \qed \; dy/dt+p(t)y=g(t) \implies y=(\int u(t)g(t))/u(t) + c$ where $u(t)=$exp$(\int p(t)dt) \qed \; y'=x; x'=y \implies x=c_1 \cosh t + c_2 \sinh t, y=c_1\sinh t+c_2 \cosh t$ or $x=c_1e^t+c_2e^{-t}, y=c_1e^t-c_2e^{-t} \qed \; y'=-x; x'=y \implies y=c_1 \cos t + c_2 \sin t, x=c_1\sin t-c_2 \cos t \qed \; x'=x+y; y'=-x+y \implies x=e^t(c_1 \cos t+c_2 \sin t); y=e^t(-c_1\sin t +c_2 \cos t) \qed \; v'=\gamma v, v(z,0)=u_0 \implies v=u_0e^{\gamma t} \qed$
{\bf Integrals: }
\begin{align*}
&\int (a+bx)\cos(kx)dx=\frac{(a+bx)\sin(kx)}{k}+\frac{bcos(kx)}{k^2}+C\\
&\int (a+bx)\sin(kx)dx=\frac{b\sin(kx)}{k^2}-\frac{(a+bx)cos(kx)}{k}+C\\
&\int (a+bx)e^{ikx}dx=\frac{e^{ikx}(b-ik(a+bx))}{k^2}+C\\
\end{align*}