\begin{solution}
By doing some problems on my own, including the examples in class and more complex ones, I came to the general "rule" that if we use the Taylor table to obtain the approximation of the $k-th$ derivative using $n$ nodes, $n>k$, we will obtain an approximation with a leading order error term of order $n-k$ and we will need up to the $n-th$ derivative in the Taylor table. For our case in this problem, since we want to approximate the second derivative at a point $x_i$ using three nodes, we will obtain a first order approximation and we will need up to the third derivative in the Taylor table. We will check that this is true at the end of the problem.
We start by showing the Taylor expansions of the function $f$ at the three points of interest,
\begin{align*}
&f_{i-2}=f(x_i-2h)=f_i-2hf'_i+\frac{4h^2}{2}f''_i-\frac{8h^3}{6}f'''_i+...\\
&f_{i}=f(x_i)=f_i\\
&f_{i+1}=f(x_i+h)=f_i+hf'_i+\frac{h^2}{2}f''_i+\frac{h^3}{6}f'''_i+...
\end{align*}
Using these expansion we can easily fill the following Taylor table.

\begin{table}[H]
\centering
\begin{tabular}{l|c c c c }
%\hline
%\multicolumn{3}{|c|}{Datos}\\
  & $f_i$ & $f'_i$ & $f''_i$ & $f'''_i$\\
\hline
$f''_i$ & $0$ & $0$ & $1$ & $0$\\
$af_{i-2}$ & $a$ & $-2ah$ & $2ah^2$ & $-8a\frac{h^3}{6}$\\
$bf_i$ & $b$ & $0$ & $0$ & $0$\\
$cf_{i+1}$ & $c$ & $ch$ & $\frac{1}{2}ch^2$ & $c\frac{h^3}{6}$\\
\end{tabular}
\caption{Taylor table.}
\end{table}

From the table above we can obtain the following system of equations,
\begin{align*}
a+b+c&=0,\\
c-2a&=0,\\
1+2ah^2+\frac{1}{2}ch^2&=0.
\end{align*}
From the second equation we know that $c=2a$, and inserting it in the third one get
\begin{align*}
1+2ah^2+ah^2=1+3ah^2=0,
\end{align*}
which gives us 
\begin{align*}
a=-\frac{1}{3h^2}~~\Rightarrow~~c=-\frac{2}{3h^2}.
\end{align*}
Finally, plugging this values in the first equation we get
\begin{align*}
-\frac{1}{3h^2}+b-\frac{2}{3h^2}=b-\frac{1}{h^2}=0,
\end{align*}
which gives us 
\begin{align*}
b=\frac{1}{h^2}.
\end{align*}
Inserting the constants in the equation
\begin{align*}
f''_i+af_{i-2}+bf_i+cf_{i+1}=(a+b+c)f_i+(c-2a)hf'_i+(1+2ah^2+\frac{1}{2}ch^2)f''_i+(c-8a)\frac{h^3}{6}f'''_i+...
\end{align*}
we obtain the desired approximation
\begin{align*}
f''_i=\frac{f_{i-2}-3f_i+2f_{i+1}}{3h^2}+\frac{h}{3}f'''_i+...
\end{align*}
where the terms of $f_i,f'_i$ and $f''_i$ of the right side of the equation have vanished. Thus, the approximation is of first order, since the leading order error term $\frac{h}{3}f'''_i$ is proportional to $h$. The aproximation can then be expressed as
\begin{align*}
f''_i=\frac{f_{i-2}-3f_i+2f_{i+1}}{3h^2}+\mathcal{O}(h).
\end{align*}
\end{solution}