{\bf Green's function (GF)} HE w/ 0 BCs, $(\partial_t - a \partial_x^2)u = 0$, on $[0,L] \times (0, \infty), u(x,0)= f(x), 0 \leq x \leq L, u(0,t) = 0 = u(L, t), t > 0$ (5.25), is given by the Fourier sine series $u(x,t) = \sum_{m=1}^{\infty} B_m e^{-a \lambda_m^2 t} \sin(\lambda_m x), \lambda_m = m \pi / L = m \lambda_1, B_m = 2/L \int_0^L f(y) \sin(\lambda_m y) dy$ (5.26). Sub 3rd into  1st eq, $u(x,t) = \sum_{m=1}^{\infty} (2/L \int_0^L f(y) \sin(\lambda_m y) dy) e^{-a \lambda_m^2 t} \sin(\lambda_m x)$. Interchange series and int, $u(x,t) = \int_0^L G(x,y,t)f(y) dy, G(x,y,t)=\sum_{m=1}^{\infty} G_m(x,y,t), t \in (0, \infty), x,y, \in [0, L]$, $G_m(x,y,t) = (2/L) \sin(\lambda_m x) \sin(\lambda_m y)e^{-a \lambda_m^2 t}$ (5.27). Notice $|\partial_x^j \partial_y^k \partial_t^{\ell} G_m(x,y,t)| \leq (2/L) a^{\ell} \lambda_m^{j+k+2\ell} e^{-a \lambda_m^2 t}$ (5.28). From ratio test, for $t > 0, \sum_{m=1}^{\infty}(2/L) a^{\ell} \lambda_m^{j+k+2\ell} e^{-a \lambda_m^2 t} < \infty$.
By T 5.2, $G$ is inf often diff on $[0, L]^2 \times (0, \infty)$ and $\partial_x^j \partial_y^k \partial_t^{\ell} G(x,y,t) = \sum_{m=1}^{\infty} \partial_x^j \partial_y^k \partial_t^{\ell} G_m(x,y,t)$ (5.29). This justifies (5.27). Also $|\partial_x^j \partial_y^k \partial_t^{\ell} G(x,y,t)| \leq \sum_{m=1}^{\infty} (2/L) a^{\ell}$
$\lambda_m^{j+k+2\ell} e^{-a \lambda_m^2 t} < \infty$ (5.30). $G$ satisfies HE because each $G_m$ does, $\partial_t G(x,y,t) = a \partial_x^2 G(x,y,t) = a \partial_y^2 G(x,y,t), 0 = G(0,y,t) = G(L,y,t)=G(x,0,t) = G(x,L,t), 0 \leq x, y \leq L, t > 0$ (5.31). From (5.27), $G(x,y,t)=G(y,x,t), 0 \leq x, y \leq L, t > 0$ (5.32). 