{\bf E5.4.4}. Let $F: [0,L]\times [0,T) \ra \R$ be cont. Define $u(x,t)= \int_0^t \int_0^L G(x,y,t-s)F(y,s)dy ds,  0 < t < T,  0 \leq x \leq L.$ Show:  For every twice contly diff $\phi: [0,L] \ra \R$ with $\phi(0) = 0 = \phi(L), \int_0^L \phi(x)u(x,t)dx$ is diff in $t \in (0,T)$ and $d/dt \int_0^L  \phi(x) u(x,t) dx = \int_0^L  a\phi''(x)u(x,t)dx + \int_0^L  \phi(x)F(x,t)dx, \quad 0 < t < T.$ Hint:  Notice and prove that $ \int_0^L  \phi(x)u(x,t)dx = \int_0^L ( \int_0^t v(y,t-s) F(y,s)ds) dy$ with $v(y,t) =  \int_0^L  \phi(x)G(x,y,t)dy = \int_0^L  G(y,z,t)\phi(z)dz,  t>0, y \in [0,L]$ (5.45), and use E 5.3.4.  You may interchange int and diff and use Leibnitz rule without prf. 
{\it Prf}. Changing the order of int, we obtain $\int_0^L \phi(x) u(x,t) dx = \int_0^L \phi(x)( \int_0^t \int_0^L G(x,y,t-s) F(y,s)ds dy )dx$ =  $\int_0^L \int_0^t (\int_0^L G(x,y,t-s)\phi(x) dx) F(y,s)ds dy$ =  $\int_0^L (\int_0^t v(y,t-s) F(y,s)ds) dy$ (5.46) with $v$ in (5.45). Recall that $G(x,y,t) = G(y,x,t)$. By E 5.3.4, $\partial_t v(y,t) = \int_0^L G(y,z,t) a \phi''(z) dz \; \exists$ and is cont for $t > 0, y \in [0,L]$ and is bdd on $[0,L] \times [0, \infty)$ because $\phi''$ is bdd on $(0, L)$ and $\int_0^L G(y,z,t) dz \leq 1$. Further $v$ can be cont extended to $[0, L] \times [0, \infty)$ with $v(y,0) = \phi(y)$. So we can apply Leibnitz rule and obtain $\partial_t \int_0^t v(y,t-s) F(y,s)ds  =  v(y,0) F(y,t) + \int_0^t \partial_t v(y,t-s) F(y,s))ds$ = $\phi(y) F(y,t) + \int_0^t ( \int_0^L G(y,z,t) a \phi''(z))F(y,s)ds$.  We interchange diff and int in (5.46), $\partial_t \int_0^L \phi(x) u(x,t)dx = \int_0^L \partial_t ( \int_0^t v(y,t-s)F(y,s)ds)dy$ = $\int_0^L (\phi(y) F(y,t) + \int_0^t ( \int_0^L G(y,z,t-s) a \phi''(z)dz ) F(y,x) ds) dy$.  We change the order of int back and use $G(y,z,t-s) = G(z,y,t-s), \partial_t \int_0^L \phi(x) u(x,t)dx = \int_0^L \phi(x) F(y,t)dy + \int_0^L a \phi''(z)u(z,t)dz \qed$
