{\bf E 6.2.2}. (a) Let $|x|$ be the Euclidean norm of $x \in \R^n$. Show: $\Delta |x| = (n-1)/|x|\; \forall \; x \in \R^n, \; x \neq 0.$ (b) Let $y \in \R^n$ be fixed and define $u: \R^n \ra \R$ by $u(x) = (|y|^2 - |x|^2)|x-y|^{-n}$.  Show that $\Delta u(x) = 0\; \forall \; x \in \R^n, x \neq y$. {\it Prf}. (a) We diff once wrt $x_j$ and get $\partial_j |x| = \partial_j (\sum_{j=1}^n x_j^2)^{1/2} = 2 x_j 1/2 (\sum_{j=1}^n x_j^2)^{-1/2} = x_j/|x|$. Now we diff again wrt $x_j, \partial_j^2 |x| =  \partial_j x_j/|x|= \partial_j x_j (\sum_{j=1}^n x_j^2)^{-1/2} =  -x_j/2 (\sum_{j=1}^n x_j^2 )^{-3/2}(2 x_j)+(\sum_{j=1}^n x_j^2)^{-1/2} = 1/|x|- x_j^2/|x|^3.$  Sum over $j$ to get $ \Delta |x| = n/|x| - |x|^2 / |x|^3 = (n-1) / |x|.$  (b) Take the first PD wrt $x_j,
\partial_j u(x) = (|y|^2 - |x|^2)(-n)|x-y|^{(-n-1)}(1/2)(\sum_{j=1}^n(x_j-y_j)^2)^{-3/2}(2x_j-2y_j) - 2 x_j |x-y|^{-n} = - 2 x_j |x-y|^{-n}-n(|y|^2 - |x|^2)|x-y|^{(-n-2)}(x_j-y_j).$ Now we diff wrt $x_j, \partial_j^2 u(x) = -2|x-y|^{-n} + 2n x_j|x-y|^{(-n-2)}(x_j-y_j)+ 2 x_j n |x-y|^{(-n-2)}(x_j-y_j) + n(n+2)(|y|^2 - |x|^2)|x-y|^{(-n-4)}(x_j-y_j)^2- n (|y|^2 - |x|^2)|x-y|^{(-n-2)}.$  Sum over $j=1, \dots, n$ and define the inner product $\langle x, y \rangle = \sum_{j=1}^nx_jy_j, \Delta u(x) = -2n|x-y|^{-n} + 4n|x-y|^{(-n-2)}\langle x, x-y \rangle  + n (n+2) (|y|^2 - |x|^2)|x-y|^{(-n-4)}|x-y|^2 - n^2(|y|^2 - |x|^2)|x-y|^{(-n-2)}.$ Simplify $\Delta u(x) = -2n|x-y|^{-n} + 4n|x-y|^{(-n-2)}\langle x, x-y \rangle +2n(|y|^2 - |x|^2)|x-y|^{(-n-2)}.$ Factor out $2n|x-y|^{(-n-2)}$ to get $\Delta u(x) = 2n|x-y|^{(-n-2)} (-|x-y|^2 + 2\langle x, x-y \rangle +|y|^2 - |x|^2) = 0 \qed$
